Proving vcs_good in UseCell.v
--HG--
branch : adt

platform/cito/ProgramLogic.v
@@ -17,7 +17,7 @@ Module Make (Import E : ADT).
 
     (* shallow embedding *)
     Definition assert := Env -> State -> State -> Prop.
-    Definition interp (p : assert) (env : Env) (v v' : State) : Prop := p env v v'.
+    Definition entailment := Env -> Prop.
 
     Inductive StmtEx := 
     | SkipEx : StmtEx
@@ -29,9 +29,9 @@ Module Make (Import E : ADT).
     | CallEx : option string -> Expr -> list Expr -> StmtEx
     | LabelEx : string -> glabel -> StmtEx.
 
-    Definition and_lift (a b : assert) : assert := fun env v v' => interp a env v v' /\ interp b env v v'.
-    Definition or_lift (a b : assert) : assert := fun env v v' => interp a env v v' \/ interp b env v v'.
-    Definition imply_close (a b : assert) : Prop := forall env v v', interp a env v v' -> interp b env v v'.
+    Definition and_lift (a b : assert) : assert := fun env v v' => a env v v' /\ b env v v'.
+    Definition or_lift (a b : assert) : assert := fun env v v' => a env v v' \/ b env v v'.
+    Definition imply_close (a b : assert) : entailment := fun env => forall v v', a env v v' -> b env v v'.
 
     Infix "/\" := and_lift : assert_scope.
     Infix "\/" := or_lift : assert_scope.
@@ -70,11 +70,11 @@ Module Make (Import E : ADT).
         | _ =>
           (fun env v0 v' =>
              exists v,
-               interp p env v0 v /\
+               p env v0 v /\
                RunsTo env stmt v v')%type
       end.
 
-    Fixpoint vc stmt (p : assert) : list Prop :=
+    Fixpoint vc stmt (p : assert) : list entailment :=
       match stmt with
         | SeqEx a b => vc a p ++ vc b (sp a p)
         | IfEx e t f => vc t (p /\ is_true e) ++ vc f (p /\ is_false e)
@@ -86,30 +86,28 @@ Module Make (Import E : ADT).
         | _ => (p --> (fun env _ v => Safe env stmt v)) :: nil
       end.
     
-    Definition and_all := fold_right and True.
+    Definition and_all : list entailment -> entailment := fold_right (fun a b env => a env /\ b env)%type (fun _ => True).
 
     Require Import GeneralTactics.
 
-    Lemma and_all_app : forall ls1 ls2, and_all (ls1 ++ ls2) -> and_all ls1 /\ and_all ls2.
+    Lemma and_all_app : forall ls1 ls2 env, and_all (ls1 ++ ls2) env -> and_all ls1 env /\ and_all ls2 env.
       induction ls1; simpl; intuition.
       eapply IHls1 in H1; openhyp; eauto.
       eapply IHls1 in H1; openhyp; eauto.
     Qed.
 
-    Lemma is_true_intro : forall e env v v', wneb (eval (fst v') e) $0 = true -> interp (is_true e) env v v'.
+    Lemma is_true_intro : forall e env v v', wneb (eval (fst v') e) $0 = true -> (is_true e) env v v'.
       intros.
       unfold is_true.
-      unfold interp.
       unfold wneb in *.
       destruct (weq _ _) in *; intuition.
     Qed.
 
     Hint Resolve is_true_intro.
 
-    Lemma is_false_intro : forall e env v v', wneb (eval (fst v') e) $0 = false -> interp (is_false e) env v v'.
+    Lemma is_false_intro : forall e env v v', wneb (eval (fst v') e) $0 = false -> (is_false e) env v v'.
       intros.
       unfold is_false.
-      unfold interp.
       unfold wneb in *.
       destruct (weq _ _) in *; intuition.
     Qed.
@@ -131,7 +129,7 @@ Module Make (Import E : ADT).
         | H : _ = _ |- _ => unfold_all; injection H; intros; subst
       end.
 
-    Lemma sound_runsto' : forall env (s : Stmt) v v', RunsTo env s v v' -> forall s' : StmtEx, s = s' -> forall p, and_all (vc s' p) -> forall v0, interp p env v0 v -> interp (sp s' p) env v0 v'.
+    Lemma sound_runsto' : forall env (s : Stmt) v v', RunsTo env s v v' -> forall s' : StmtEx, s = s' -> forall p, and_all (vc s' p) env -> forall v0, p env v0 v -> (sp s' p) env v0 v'.
       induction 1; simpl; intros; destruct s'; try discriminate; simpl in *; try inject.
 
       (* skip *)
@@ -166,26 +164,26 @@ Module Make (Import E : ADT).
 
       Focus 4.
       (* assign *)
-      unfold interp; eauto.
+      eauto.
 
       Focus 3.
       (* label *)
-      unfold interp; eauto.
+      eauto.
 
       (* call *)
-      unfold interp; eauto.
-      unfold interp; eauto.
+      eauto.
+      eauto.
     Qed.
 
-    Theorem sound_runsto : forall env (s : StmtEx) v v' p v0, RunsTo env s v v' -> and_all (vc s p) -> interp p env v0 v -> interp (sp s p) env v0 v'.
+    Theorem sound_runsto : forall env (s : StmtEx) v v' p v0, RunsTo env s v v' -> and_all (vc s p) env -> p env v0 v -> (sp s p) env v0 v'.
       intros.
       eapply sound_runsto'; eauto.
     Qed.
 
-    Theorem sound_safe : forall env (s : Stmt) (s' : StmtEx) v p v0, s = s' -> and_all (vc s' p) -> interp p env v0 v -> Safe env s v.
+    Theorem sound_safe : forall env (s : Stmt) (s' : StmtEx) v p v0, s = s' -> and_all (vc s' p) env -> p env v0 v -> Safe env s v.
       intros.
       Close Scope assert_scope.
-      eapply (Safe_coind (fun s v => Safe env s v \/ exists (s' : StmtEx) p v0, s = s' /\ and_all (vc s' p) /\ interp p env v0 v)); [ .. | right; descend; eauto]; clear; intros; openhyp.
+      eapply (Safe_coind (fun s v => Safe env s v \/ exists (s' : StmtEx) p v0, s = s' /\ and_all (vc s' p) env /\ p env v0 v)); [ .. | right; descend; eauto]; clear; intros; openhyp.
 
       (* seq *)
       inversion H; subst.
@@ -259,7 +257,6 @@ Module Make (Import E : ADT).
       destruct x; try discriminate; simpl in *; try inject.
       openhyp.
       eapply H0 in H1.
-      unfold interp in *.
       inversion H1; unfold_all; subst.
       left; descend; eauto.
       right; descend; eauto.
@@ -270,7 +267,6 @@ Module Make (Import E : ADT).
 
       destruct x0; try discriminate; simpl in *; try inject.
       eapply H0 in H1.
-      unfold interp in *.
       inversion H1; unfold_all; subst.
       eauto.
     Qed.
